Checking in some work in progress.

hol/pc-verification/forparConvertScript.sml
@@ -11,6 +11,8 @@ open PseudoCHDAGTheory
 open monadsyntax boolSimps
 open lcsymtacs
 
+open indexedListsTheory
+
 val _ = new_theory "forparConvert";
 
 val _ = set_trace "Goalstack.print_goal_at_top" 0
@@ -67,17 +69,152 @@ val graphOf_ForLoop_Seq = store_thm(
         (Int lo_i, Int hi_i) => if lo_i <= hi_i then
 *)
 
-val domreadAction_write = store_thm(
-  "domreadAction_write[simp]",
-  ``(domreadAction l m d).write = NONE``,
-  Cases_on `d` >> simp[domreadAction_def]);
+val _ = augment_srw_ss [intSimps.OMEGA_ss]
+
+val strip_labels_def = Define`
+  strip_labels (g : 'a pcg) : unit pcg = hdmap (K () ## I) g
+`
+
+val nstrip_labels_def = Define`
+  nstrip_labels (n : 'a pcnode) : unit pcnode = nmap (K () ## I) n
+`;
+
+val strip_labels_thm = store_thm(
+  "strip_labels_thm[simp]",
+  ``strip_labels ε = ε ∧
+    strip_labels (n <+ g) = nstrip_labels n <+ strip_labels g ∧
+    nstrip_labels (HD a) = HD (polydata_upd (K () ## I) a) ∧
+    nstrip_labels (HG g) = HG (strip_labels g)``,
+  simp[strip_labels_def, nstrip_labels_def]);
+
+val polydata_upd_o = store_thm(
+  "polydata_upd_o[simp]",
+  ``polydata_upd f (polydata_upd g a) = polydata_upd (f o g) a``,
+  simp[actionTheory.polydata_upd_def]);
+
+val SND_PAIRMAP = store_thm(
+  "SND_PAIRMAP[simp]",
+  ``SND o (f ## g) = g o SND``,
+  simp[FUN_EQ_THM]);
+
+val strip_labels_preserves_meaning = store_thm(
+  "strip_labels_preserves_meaning[simp]",
+  ``(∀n: α pcnode. pcn_eval (nstrip_labels n) = pcn_eval n) ∧
+    (∀g: α pcg. pcg_eval (strip_labels g) = pcg_eval g)``,
+  ho_match_mp_tac hidag_ind >> simp[pcg_eval_thm, FUN_EQ_THM]);
+
+val strip_labels_merge = store_thm(
+  "strip_labels_merge[simp]",
+  ``∀g1 g2. strip_labels (g1 ⊕ g2) = strip_labels g1 ⊕ strip_labels g2``,
+  Induct >> simp[]);
+
+fun rename_subterm pat_t avoids t = let
+  fun test (bvs, subt) =
+      case SOME(match_term pat_t subt) handle HOL_ERR _ => NONE of
+          SOME(tmsub, tysub)
+      if can (match_term pat_t) subt then
+
+
+fun case_t (q,sl) = let
+  fun has_t (asl, w) = let
+    val t = parse_in_context (w::asl) q
+  in
+    if List.exists (free_in t) (w::asl) then ALL_TAC
+    else NO_TAC
+  end (asl,w)
+in
+  qmatch_rename_tac q sl ORELSE qmatch_assum_rename_tac q sl ORELSE
+  has_t
+end
+
+
+val hdmerge_cons_snoc = store_thm(
+  "hdmerge_cons_snoc",
+  ``∀g h a b. g ⊕ (a <+ ε) = b <+ h ⇔
+                a = b ∧ g = h ∧ ¬ngtouches a g ∨
+                ∃gh0. g = b <+ gh0 ∧ h = gh0 ⊕ (a <+ ε)``,
+  Induct >> conj_tac >> simp[] >- metis_tac[] >>
+  qx_gen_tac `g` >> strip_tac >> simp[hidagAdd_11_thm] >>
+  qx_genl_tac [`a1`, `h`, `b`, `a2`] >> Cases_on `a1 ∼ₜ a2` >> dsimp[]
+  >- metis_tac[htouches_SYM] >>
+  Cases_on `a1 = a2` >- (dsimp[EQ_IMP_THM] >> rw[] >> metis_tac[htouches_SYM]) >>
+  simp[] >> metis_tac[htouches_SYM]);
+
+val ngtouches_merge = store_thm(
+  "ngtouches_merge[simp]",
+  ``ngtouches n (g1 ⊕ g2) ⇔ ngtouches n g1 ∨ ngtouches n g2``,
+  Induct_on `g1` >> simp[]);
+
+val hdmerge_11 = store_thm(
+  "hdmerge_11[simp]",
+  ``(∀g g1 g2. g ⊕ g1 = g ⊕ g2 ⇔ g1 = g2) ∧
+    (∀g g1 g2. g1 ⊕ g = g2 ⊕ g ⇔ g1 = g2)``,
+  conj_tac >> Induct >> simp[] >> rpt strip_tac >>
+  `∀a g1. g1 ⊕ a <+ g = (g1 ⊕ a <+ ε) ⊕ g`
+    by (Induct_on `g1` >> simp[]) >>
+  pop_assum (fn th => ONCE_REWRITE_TAC [th]) >>
+  simp[] >> pop_assum kall_tac >> map_every qid_spec_tac [`g2`, `g1`] >>
+  Induct >> simp[] >> rpt strip_tac >- (Cases_on `g2` >> simp[]) >>
+  qmatch_rename_tac `b <+ (g1 ⊕ a <+ ε) = g2 ⊕ a <+ ε ⇔ b <+ g1 = g2` [] >>
+  dsimp[hdmerge_cons_snoc, EQ_IMP_THM] >> rw[] >> fs[]);
+
+(*
+val graphOf_label_invariant = store_thm(
+  "graphOf_label_invariant",
+  ``∀s lab m0 m g.
+      graphOf lab m0 s = SOME(m,g) ⇒
+      ∀lab'.
+        ∃g'. graphOf lab' m0 s = SOME(m,g') ∧
+             strip_labels g' = strip_labels g``,
+  ho_match_mp_tac graphOf_ind' >> Cases >> strip_tac >>
+  TRY (simp_tac (srw_ss()) [Once graphOf_def] >> NO_TAC) >>
+  FIRST [
+
+  has_t `Assign` >>
+    simp[graphOf_def, PULL_EXISTS, mareadAction_def, actionTheory.polydata_upd_def,
+         dvreadAction_def, addLabel_def],
+
+  has_t `IfStmt` >>
+    dsimp[graphOf_def, value_case_eq, PULL_EXISTS, bool_case_eq, EXISTS_PROD,
+          addLabel_def, readAction_def, actionTheory.polydata_upd_def] >>
+    fs[AND_IMP_INTRO, PULL_FORALL] >> rpt strip_tac >> first_x_assum match_mp_tac >>
+    simp[pairTheory.LEX_DEF, MAX_PLUS] >> metis_tac[],
+
+  has_t `ForLoop` >>
+    simp[graphOf_def, PULL_EXISTS, EXISTS_PROD, FORALL_PROD, addLabel_def,
+         actionTheory.polydata_upd_def] >>
+    qx_genl_tac [`lab`, `m0`, `m`, `dvs`, `g`] >> strip_tac >>
+    Q.UNDISCH_THEN `dvalues m0 d = SOME dvs` kall_tac >>
+    fs[rich_listTheory.FOLDL_FOLDR_REVERSE] >>
+    qabbrev_tac `ds = REVERSE dvs` >> markerLib.RM_ALL_ABBREVS_TAC >>
+    pop_assum mp_tac >> map_every qid_spec_tac [`m`, `g`] >>
+    Induct_on `ds` >> simp[PULL_EXISTS, FORALL_PROD, EXISTS_PROD] >>
+    qabbrev_tac `ff = λlab vnm bod v mg0.
+       do
+          (m0', g0) <- mg0;
+          (m, g') <- graphOf (v::lab) m0' (ssubst vnm v bod);
+          SOME(m, g0 ⊕ HG g' <+ ε)
+       od` >> fs[] >>
+    full_simp_tac (srw_ss() ++ ETA_ss) [] >> rpt strip_tac >>
+    res_tac >> first_x_assum (qspec_then `lab'` strip_assume_tac) >>
+    simp[] >> fs[PULL_FORALL, AND_IMP_INTRO] >>
+    first_x_assum match_mp_tac >> simp[pairTheory.LEX_DEF] >> rw[] >>
+    metis_tac[],
+
+  has_t `ParLoop` >>
+    simp[graphOf_def, PULL_EXISTS, addLabel_def, combinTheory.o_ABS_R]
+
+  ALL_TAC
+  ]
+
+*)
 
 val simple_executor_equivalence = store_thm(
   "simple_executor_equivalence",
   ``evalexpr m0 lo = Int loi ∧
     evalexpr m0 hi = Int hii ∧
     wave_array_correct wave_a loi hii g m0 ∧
-    w ≠ i ∧ wave_a ≠ i ∧ wave_a ≠ w ∧ w # lo ∧ w # hi ∧
+    w ≠ i ∧ wave_a ≠ i ∧ wave_a ≠ w ∧ w # lo ∧ w # hi ∧ w # body ∧
     graphOf [] m0 (ForLoop i (D lo hi) body) = SOME(m,g) ⇒
     ∃g'.
       graphOf [] m0
@@ -88,7 +225,7 @@ val simple_executor_equivalence = store_thm(
               (IfStmt (ARead wave_a (VarExpr i) == VarExpr w)
                       body
                       Done))) = SOME(m,g') ∧
-      strip_purereads g' = g``,
+      strip_labels (strip_purereads g') = strip_labels g``,
   ONCE_REWRITE_TAC [graphOf_def] >>
   csimp[dvalues_def, evalexpr_def, PULL_EXISTS, EXISTS_PROD,
         FORALL_PROD, ssubst_def, esubst_def] >>
@@ -96,7 +233,12 @@ val simple_executor_equivalence = store_thm(
        REVERSE_GENLIST, combinTheory.o_ABS_R,
        DECIDE ``PRE n - m = n - (m + 1)``] >>
   qx_gen_tac `g0` >> strip_tac >>
-  `loi ≤ hii` by fs[wave_array_correct_def] >> fs[]
+  `loi ≤ hii` by fs[wave_array_correct_def] >> fs[] >>
+  qabbrev_tac `sz = Num (hii - loi)` >>
+  `∀m. m < sz ⇒ &(sz - (m + 1)) + loi = hii - &(m + 1)`
+    by simp[int_arithTheory.INT_NUM_SUB, Abbr`sz`] >>
+  fs[Cong GENLIST_CONG] >>
+  simp[graphOf_def, ssubst_def, esubst_def]
  );
 
 val _ = export_theory();
